okasaki/CatenableListImpl_proof.v
@@ -1,0 +1,144 @@
+Set Implicit Arguments.
+Require Import FuncTactics LibCore.
+Require Import DequeSig_ml DequeSig_proof.
+Require Import BankersDeque_ml.
+
+Module CatenableListImplSpec (Q:MLQueue) (QS:QueueSigSpec with Module Q:=Q)
+  <: CatenableListSigSpec.
+
+(** instantiations *)
+
+Module Import C <: MLCatenableList := MLCatenableListImpl.
+Import MLCatenableListImpl.
+
+(** invariant *)
+
+Inductive inv `{Rep a A} (c:cat a) (L:list A) :=
+  | inv_empty :
+      inv Empty nil
+  | inv_struct : forall x q X Ls L,
+      rep x X ->
+      rep (H := Build_Rep inv) q Ls ->
+      L =' X :: Ls ->
+      Forall (<> nil) Ls.
+      
+Global Instance deque_rep `{Rep a A} : Rep (cat a) (list A) :=
+  inv 0.
+
+(** automation *)
+
+Hint Constructors Forall2.
+Hint Resolve Forall2_last.
+Hint Extern 1 (@rep (cat _) _ _ _ _) => simpl.
+Hint Unfold inv.
+
+Ltac auto_tilde ::= eauto with maths.
+
+Section Polymorphic.
+Variables (a A : Type) (RA:Rep a A).
+
+  (* todo: avoid the following lines *)
+Hint Extern 1 (RegisterSpec Q.is_empty) => Provide (QS.is_empty_spec (H:=RA)).
+Hint Extern 1 (RegisterSpec Q.snoc) => Provide (QS.snoc_spec (H:=RA)).
+Hint Extern 1 (RegisterSpec Q.head) => Provide (QS.head_spec (H:=RA)).
+Hint Extern 1 (RegisterSpec Q.tail) => Provide (QS.tail_spec (H:=RA)).
+
+(** useful facts *)
+
+Lemma to_empty : forall L,
+  rep Empty L -> L = nil.
+Proof. introv RL. inverts RL as _ M. inverts~ M. Qed.
+
+Lemma to_not_empty : forall c L,
+  rep c L -> L <> nil -> c <> Empty.
+Proof.
+  introv RL NE K. subst. apply NE. apply~ to_empty.
+Qed.
+
+Lemma from_empty : forall c,
+  rep c nil -> c = Empty.
+Proof.
+  introv RC. inverts RC as.
+  introv _ ID. inverts~ ID.
+  introv ? ? Df ? ? ?. inverts Df; false.
+Qed.
+
+(** verification *)
+
+Lemma empty_spec : 
+  rep (@empty a) (@nil A).
+Proof.
+  generalizes RA A. apply (empty_cf a). xgo.
+  intros. simpl. rew_list~.
+Qed.
+
+Hint Extern 1 (rep empty _) => apply empty_spec.
+
+Lemma is_empty_spec : 
+  RepTotal is_empty (L;cat a) >> bool_of (L = nil).
+Proof.
+  xcf. intros (((lenf,f),lenr),r) Q RQ. xgo.
+  unfolds. extens. iff Z; fold_prop; subst.
+  apply~ empty_from_len.
+  intuit RQ. inverts H. destruct (nil_eq_app_rev_inv H5). subst~.
+Qed. 
+
+Hint Extern 1 (RegisterSpec is_empty) => Provide is_empty_spec.
+
+Lemma link_spec : 
+  RepSpec link (L1;cat a) (L2;cat a) |R>>
+    L1 <> nil -> L2 <> nil -> R (L1 ++ L2 ; cat a).
+Proof.
+Qed.
+
+Hint Extern 1 (RegisterSpec link) => Provide link_spec.
+
+Lemma link_all_spec : 
+  RepSpec link_all (Ls;queue (cat a)) |R>>
+    Ls <> nil -> R (concat Ls ; cat a).
+Proof.
+Qed.
+
+Hint Extern 1 (RegisterSpec link_all) => Provide link_all_spec.
+
+Lemma append_spec : 
+  RepTotal append (L1;cat a) (L2;cat a) >> (L1++L2) ; cat a.
+Proof.
+Qed.
+
+Hint Extern 1 (RegisterSpec append) => Provide append_spec.
+
+Lemma cons_spec : 
+  RepTotal cons (X;a) (L;cat a) >> (X::L) ; cat a.
+Proof.
+Qed.
+
+Hint Extern 1 (RegisterSpec cons) => Provide cons_spec.
+
+Lemma snoc_spec : 
+  RepTotal snoc (L;cat a) (X;a) >> (L&X) ; cat a.
+Proof.
+Qed.
+
+Hint Extern 1 (RegisterSpec snoc) => Provide snoc_spec.
+
+Lemma head_spec : 
+  RepSpec head (L;cat a) |R>>
+     L <> nil -> R (is_head L ;; a).
+Proof.
+Qed.
+
+Hint Extern 1 (RegisterSpec head) => Provide head_spec.
+
+Lemma tail_spec :
+  RepSpec tail (L;cat a) |R>> 
+     L <> nil -> R (is_tail L ;; cat a).
+Proof.
+Qed.
+
+Hint Extern 1 (RegisterSpec tail) => Provide tail_spec.
+
+End Polymorphic.
+
+End CatenableListImplSpec.
+
